WIP

src/Init/Data/String/Lemmas/g.lean
@@ -130,26 +130,26 @@ def ofSliceFrom {s : Slice} {p : s.Pos} (st : SearchStep (s.sliceFrom p)) : Sear
 
 end SearchStep
 
-structure IsMatchList (s : Slice) (l : List (SearchStep s)) : Prop where
-  exists_le_and_lt : ∀ p : s.Pos, p ≠ s.endPos → ∃ st ∈ l, st.startPos ≤ p ∧ p < st.endPos
-  lt : ∀ st ∈ l, st.startPos < st.endPos
-  isChain : l.IsChain (fun l r => l.endPos = r.startPos)
+-- structure IsMatchList (s : Slice) (l : List (SearchStep s)) : Prop where
+--   exists_le_and_lt : ∀ p : s.Pos, p ≠ s.endPos → ∃ st ∈ l, st.startPos ≤ p ∧ p < st.endPos
+--   lt : ∀ st ∈ l, st.startPos < st.endPos
+--   isChain : l.IsChain (fun l r => l.endPos = r.startPos)
 
-theorem IsMatchList.eq_nil_iff {s : Slice} {l : List (SearchStep s)} (h : IsMatchList s l) :
-    l = [] ↔ s.isEmpty := by
-  refine ⟨?_, ?_⟩
-  · rintro rfl
-    rw [← startPos_eq_endPos_iff]
-    refine Classical.not_not.1 (fun h' => ?_)
-    simpa using h.exists_le_and_lt s.startPos h'
-  · rw [← Decidable.not_imp_not]
-    intro hl
-    simp only [Bool.not_eq_true]
-    exact Slice.isEmpty_eq_false_of_lt (h.lt _ (List.head_mem hl))
+-- theorem IsMatchList.eq_nil_iff {s : Slice} {l : List (SearchStep s)} (h : IsMatchList s l) :
+--     l = [] ↔ s.isEmpty := by
+--   refine ⟨?_, ?_⟩
+--   · rintro rfl
+--     rw [← startPos_eq_endPos_iff]
+--     refine Classical.not_not.1 (fun h' => ?_)
+--     simpa using h.exists_le_and_lt s.startPos h'
+--   · rw [← Decidable.not_imp_not]
+--     intro hl
+--     simp only [Bool.not_eq_true]
+--     exact Slice.isEmpty_eq_false_of_lt (h.lt _ (List.head_mem hl))
 
-class LawfulToForwardSearcher {ρ : Type} {σ : Slice → Type} (pat : ρ) [ToForwardSearcher pat σ]
-    [∀ s, Std.Iterator (σ s) Id (SearchStep s)] [∀ s, Std.Iterators.Finite (σ s) Id] where
-  isMatchList (s : Slice) : IsMatchList s (ToForwardSearcher.toSearcher pat s).toList
+-- class LawfulToForwardSearcher {ρ : Type} {σ : Slice → Type} (pat : ρ) [ToForwardSearcher pat σ]
+--     [∀ s, Std.Iterator (σ s) Id (SearchStep s)] [∀ s, Std.Iterators.Finite (σ s) Id] where
+--   isMatchList (s : Slice) : IsMatchList s (ToForwardSearcher.toSearcher pat s).toList
 
 class LawfulToForwardSearcher₂ {ρ : Type} {σ : Slice → Type} (pat : ρ) [ToForwardSearcher pat σ]
     [∀ s, Std.Iterator (σ s) Id (SearchStep s)] [∀ s, Std.Iterators.Finite (σ s) Id] where
@@ -160,24 +160,24 @@ class LawfulToForwardSearcher₂ {ρ : Type} {σ : Slice → Type} (pat : ρ) [T
       (ToForwardSearcher.toSearcher pat s).toList = st ::
         (ToForwardSearcher.toSearcher pat (s.sliceFrom st.endPos)).toList.map SearchStep.ofSliceFrom
 
-theorem toList_toSearcher_eq_nil_iff {ρ : Type} {σ : Slice → Type} {pat : ρ}
-    [ToForwardSearcher pat σ]
-    [∀ s, Std.Iterator (σ s) Id (SearchStep s)] [∀ s, Std.Iterators.Finite (σ s) Id]
-    [LawfulToForwardSearcher pat] :
-    (ToForwardSearcher.toSearcher pat s).toList = [] ↔ s.isEmpty :=
-  (LawfulToForwardSearcher.isMatchList s).eq_nil_iff
+-- theorem toList_toSearcher_eq_nil_iff {ρ : Type} {σ : Slice → Type} {pat : ρ}
+--     [ToForwardSearcher pat σ]
+--     [∀ s, Std.Iterator (σ s) Id (SearchStep s)] [∀ s, Std.Iterators.Finite (σ s) Id]
+--     [LawfulToForwardSearcher pat] :
+--     (ToForwardSearcher.toSearcher pat s).toList = [] ↔ s.isEmpty :=
+--   (LawfulToForwardSearcher.isMatchList s).eq_nil_iff
 
 class LawfulForwardPattern {ρ : Type} (pat : ρ) [ForwardPattern pat] : Prop where
   isSome_dropPrefix? (s : Slice) : (ForwardPattern.dropPrefix? pat s).isSome = ForwardPattern.startsWith pat s
   dropPrefix?_ne_startPos (s : Slice) (p : s.Pos) : ForwardPattern.dropPrefix? pat s = some p → p ≠ s.startPos
 
-class LawfulToForwardSearcherForwardPattern {ρ : Type} {σ : Slice → Type} (pat : ρ)
-    [ToForwardSearcher pat σ] [∀ s, Std.Iterator (σ s) Id (SearchStep s)]
-    [∀ s, Std.Iterators.Finite (σ s) Id] [ForwardPattern pat] where
-  reject_valid : ∀ l r, SearchStep.rejected l r ∈ (ToForwardSearcher.toSearcher pat s).toList →
-    ∀ q, l ≤ q ∧ q < r → ForwardPattern.startsWith pat (s.sliceFrom q) = false
-  match_valid : ∀ l r, SearchStep.matched l r ∈ (ToForwardSearcher.toSearcher pat s).toList →
-    ∃ h, ForwardPattern.dropPrefix? pat (s.sliceFrom l) = some (Slice.Pos.sliceFrom _ r h)
+-- class LawfulToForwardSearcherForwardPattern {ρ : Type} {σ : Slice → Type} (pat : ρ)
+--     [ToForwardSearcher pat σ] [∀ s, Std.Iterator (σ s) Id (SearchStep s)]
+--     [∀ s, Std.Iterators.Finite (σ s) Id] [ForwardPattern pat] where
+--   reject_valid : ∀ l r, SearchStep.rejected l r ∈ (ToForwardSearcher.toSearcher pat s).toList →
+--     ∀ q, l ≤ q ∧ q < r → ForwardPattern.startsWith pat (s.sliceFrom q) = false
+--   match_valid : ∀ l r, SearchStep.matched l r ∈ (ToForwardSearcher.toSearcher pat s).toList →
+--     ∃ h, ForwardPattern.dropPrefix? pat (s.sliceFrom l) = some (Slice.Pos.sliceFrom _ r h)
 
 class LawfulToForwardSearcherForwardPattern₂ {ρ : Type} {σ : Slice → Type} (pat : ρ)
     [ToForwardSearcher pat σ] [∀ s, Std.Iterator (σ s) Id (SearchStep s)]
@@ -197,106 +197,116 @@ theorem ForwardPattern.dropPrefix?_defaultImplementation {ρ : Type} {σ : Slice
     letI := ForwardPattern.defaultImplementation (pat := pat)
     ForwardPattern.dropPrefix? pat s = ForwardPattern.defaultDropPrefix? pat s := rfl
 
-theorem LawfulForwardPattern.defaultImplementation {ρ : Type} {σ : Slice → Type}
-    [∀ s, Std.Iterator (σ s) Id (SearchStep s)] {pat : ρ} [ToForwardSearcher pat σ]
-    [∀ s, Std.Iterators.Finite (σ s) Id] [LawfulToForwardSearcher pat]
-    [∀ s, Std.IteratorLoop (σ s) Id Id] [∀ s, Std.LawfulIteratorLoop (σ s) Id Id] :
-    letI : ForwardPattern pat := ForwardPattern.defaultImplementation (pat := pat)
-    LawfulForwardPattern pat := by
-  letI : ForwardPattern pat := ForwardPattern.defaultImplementation (pat := pat)
-  refine ⟨fun s => ?_, fun s p => ?_⟩
-  · rw [ForwardPattern.dropPrefix?_defaultImplementation,
-      ForwardPattern.startsWith_defaultImplementation,
-      ForwardPattern.defaultStartsWith, ForwardPattern.defaultDropPrefix?]
-    split <;> simp
-  · rw [ForwardPattern.dropPrefix?_defaultImplementation, ForwardPattern.defaultDropPrefix?]
-    rw [Std.Iter.first?_eq_head?_toList]
-    split
-    · rename_i o start stop h
-      simp only [Option.some.injEq]
-      rintro rfl
-      have := LawfulToForwardSearcher.isMatchList (pat := pat) s |>.lt _ (List.mem_of_head? h)
-      simp only [SearchStep.startPos_matched, SearchStep.endPos_matched] at this
-      exact Slice.Pos.ne_startPos_of_lt this
-    · simp
+theorem toList_splitIterator {ρ : Type} {σ : Slice → Type}
+    [∀ s, Std.Iterator (σ s) Id (SearchStep s)] [∀ s, Std.Iterators.Finite (σ s) Id]
+    [∀ s, Std.IteratorLoop (σ s) Id Id]
+    {pat : ρ} [ToForwardSearcher pat σ]
+    [ForwardPattern pat] [LawfulToForwardSearcher₂ pat] [LawfulToForwardSearcherForwardPattern₂ pat]
+    (s : Slice) :
+    (s.split pat).toList =
+      match s.dropPrefix? pat with
+      | some
 
-theorem LawfulToForwardSearcherForwardPattern.defaultImplementation {ρ : Type} {σ : Slice → Type}
-    [∀ s, Std.Iterator (σ s) Id (SearchStep s)] {pat : ρ} [ToForwardSearcher pat σ]
-    [∀ s, Std.Iterators.Finite (σ s) Id] [LawfulToForwardSearcher pat]
-    [∀ s, Std.IteratorLoop (σ s) Id Id] [∀ s, Std.LawfulIteratorLoop (σ s) Id Id] :
-    letI : ForwardPattern pat := ForwardPattern.defaultImplementation (pat := pat)
-    LawfulToForwardSearcherForwardPattern pat := by
-  letI : ForwardPattern pat := ForwardPattern.defaultImplementation (pat := pat)
-  refine ⟨fun {s} l r h q => ?_, ?_⟩
-  · rw [ForwardPattern.startsWith_defaultImplementation,
-      ForwardPattern.defaultStartsWith]
+-- theorem LawfulForwardPattern.defaultImplementation {ρ : Type} {σ : Slice → Type}
+--     [∀ s, Std.Iterator (σ s) Id (SearchStep s)] {pat : ρ} [ToForwardSearcher pat σ]
+--     [∀ s, Std.Iterators.Finite (σ s) Id] [LawfulToForwardSearcher pat]
+--     [∀ s, Std.IteratorLoop (σ s) Id Id] [∀ s, Std.LawfulIteratorLoop (σ s) Id Id] :
+--     letI : ForwardPattern pat := ForwardPattern.defaultImplementation (pat := pat)
+--     LawfulForwardPattern pat := by
+--   letI : ForwardPattern pat := ForwardPattern.defaultImplementation (pat := pat)
+--   refine ⟨fun s => ?_, fun s p => ?_⟩
+--   · rw [ForwardPattern.dropPrefix?_defaultImplementation,
+--       ForwardPattern.startsWith_defaultImplementation,
+--       ForwardPattern.defaultStartsWith, ForwardPattern.defaultDropPrefix?]
+--     split <;> simp
+--   · rw [ForwardPattern.dropPrefix?_defaultImplementation, ForwardPattern.defaultDropPrefix?]
+--     rw [Std.Iter.first?_eq_head?_toList]
+--     split
+--     · rename_i o start stop h
+--       simp only [Option.some.injEq]
+--       rintro rfl
+--       have := LawfulToForwardSearcher.isMatchList (pat := pat) s |>.lt _ (List.mem_of_head? h)
+--       simp only [SearchStep.startPos_matched, SearchStep.endPos_matched] at this
+--       exact Slice.Pos.ne_startPos_of_lt this
+--     · simp
 
-  · sorry
+-- theorem LawfulToForwardSearcherForwardPattern.defaultImplementation {ρ : Type} {σ : Slice → Type}
+--     [∀ s, Std.Iterator (σ s) Id (SearchStep s)] {pat : ρ} [ToForwardSearcher pat σ]
+--     [∀ s, Std.Iterators.Finite (σ s) Id] [LawfulToForwardSearcher pat]
+--     [∀ s, Std.IteratorLoop (σ s) Id Id] [∀ s, Std.LawfulIteratorLoop (σ s) Id Id] :
+--     letI : ForwardPattern pat := ForwardPattern.defaultImplementation (pat := pat)
+--     LawfulToForwardSearcherForwardPattern pat := by
+--   letI : ForwardPattern pat := ForwardPattern.defaultImplementation (pat := pat)
+--   refine ⟨fun {s} l r h q => ?_, ?_⟩
+--   · rw [ForwardPattern.startsWith_defaultImplementation,
+--       ForwardPattern.defaultStartsWith]
 
-def stupidSearch {ρ : Type} (pat : ρ) [ForwardPattern pat] [LawfulForwardPattern pat] {s : Slice}
-    (pos : s.Pos) : List (SearchStep s) :=
-  if h : pos = s.endPos then
-    []
-  else
-    match hend : ForwardPattern.dropPrefix? pat (s.sliceFrom pos) with
-    | some endPos =>
-      have : pos < Slice.Pos.ofSliceFrom endPos := by
-        refine Std.lt_of_le_of_lt (Slice.Pos.le_ofSliceFrom (pos := (s.sliceFrom pos).startPos)) ?_
-        rw [Slice.Pos.ofSliceFrom_lt_ofSliceFrom_iff]
-        simpa using LawfulForwardPattern.dropPrefix?_ne_startPos _ _ hend
-      SearchStep.matched pos (Slice.Pos.ofSliceFrom endPos) :: stupidSearch pat (Slice.Pos.ofSliceFrom endPos)
-    | none => SearchStep.rejected pos (pos.next h) :: stupidSearch pat (pos.next h)
-termination_by pos
+--   · sorry
 
-theorem head?_stupidSearch {ρ : Type} (pat : ρ) [ForwardPattern pat] [LawfulForwardPattern pat]
-    {s : Slice} (pos : s.Pos) (st : SearchStep s) :
-    (stupidSearch pat pos).head? = some st → st.startPos = pos := by
-  fun_induction stupidSearch with
-  | case1 => simp
-  | case3 => simp; rintro rfl; simp
-  | case2 => simp; rintro rfl; simp
+-- def stupidSearch {ρ : Type} (pat : ρ) [ForwardPattern pat] [LawfulForwardPattern pat] {s : Slice}
+--     (pos : s.Pos) : List (SearchStep s) :=
+--   if h : pos = s.endPos then
+--     []
+--   else
+--     match hend : ForwardPattern.dropPrefix? pat (s.sliceFrom pos) with
+--     | some endPos =>
+--       have : pos < Slice.Pos.ofSliceFrom endPos := by
+--         refine Std.lt_of_le_of_lt (Slice.Pos.le_ofSliceFrom (pos := (s.sliceFrom pos).startPos)) ?_
+--         rw [Slice.Pos.ofSliceFrom_lt_ofSliceFrom_iff]
+--         simpa using LawfulForwardPattern.dropPrefix?_ne_startPos _ _ hend
+--       SearchStep.matched pos (Slice.Pos.ofSliceFrom endPos) :: stupidSearch pat (Slice.Pos.ofSliceFrom endPos)
+--     | none => SearchStep.rejected pos (pos.next h) :: stupidSearch pat (pos.next h)
+-- termination_by pos
 
-theorem exists_le_and_lt_stupidSearch {ρ : Type} (pat : ρ) [ForwardPattern pat]
-    [LawfulForwardPattern pat] {s : Slice} (pos q : s.Pos) (hq : pos ≤ q) (hq' : q ≠ s.endPos) :
-    ∃ st ∈ stupidSearch pat pos, st.startPos ≤ q ∧ q < st.endPos := by
-  fun_induction stupidSearch with
-  | case1 => simp_all
-  | case2 x h endPos hend hlt ih =>
-    simp only [List.mem_cons, exists_eq_or_imp, SearchStep.startPos_matched,
-      SearchStep.endPos_matched]
-    by_cases hqe : q < Pos.ofSliceFrom endPos
-    · exact Or.inl ⟨hq, hqe⟩
-    · exact Or.inr (ih (Std.not_lt.1 hqe))
-  | case3 x h hend ih =>
-    simp only [List.mem_cons, exists_eq_or_imp, SearchStep.startPos_rejected,
-      SearchStep.endPos_rejected]
-    by_cases hqe : q < x.next h
-    · exact Or.inl ⟨hq, hqe⟩
-    · exact Or.inr (ih (Std.not_lt.1 hqe))
+-- theorem head?_stupidSearch {ρ : Type} (pat : ρ) [ForwardPattern pat] [LawfulForwardPattern pat]
+--     {s : Slice} (pos : s.Pos) (st : SearchStep s) :
+--     (stupidSearch pat pos).head? = some st → st.startPos = pos := by
+--   fun_induction stupidSearch with
+--   | case1 => simp
+--   | case3 => simp; rintro rfl; simp
+--   | case2 => simp; rintro rfl; simp
 
-theorem lt_of_stupidSearch {ρ : Type} (pat : ρ) [ForwardPattern pat] [LawfulForwardPattern pat]
-    {s : Slice} (pos : s.Pos) : ∀ st ∈ stupidSearch pat pos, st.startPos < st.endPos := by
-  fun_induction stupidSearch with
-  | case1 => simp
-  | case2 p hp endPos hend hlt ih => simpa using ⟨hlt, ih⟩
-  | case3 p hp hend ih => simpa
+-- theorem exists_le_and_lt_stupidSearch {ρ : Type} (pat : ρ) [ForwardPattern pat]
+--     [LawfulForwardPattern pat] {s : Slice} (pos q : s.Pos) (hq : pos ≤ q) (hq' : q ≠ s.endPos) :
+--     ∃ st ∈ stupidSearch pat pos, st.startPos ≤ q ∧ q < st.endPos := by
+--   fun_induction stupidSearch with
+--   | case1 => simp_all
+--   | case2 x h endPos hend hlt ih =>
+--     simp only [List.mem_cons, exists_eq_or_imp, SearchStep.startPos_matched,
+--       SearchStep.endPos_matched]
+--     by_cases hqe : q < Pos.ofSliceFrom endPos
+--     · exact Or.inl ⟨hq, hqe⟩
+--     · exact Or.inr (ih (Std.not_lt.1 hqe))
+--   | case3 x h hend ih =>
+--     simp only [List.mem_cons, exists_eq_or_imp, SearchStep.startPos_rejected,
+--       SearchStep.endPos_rejected]
+--     by_cases hqe : q < x.next h
+--     · exact Or.inl ⟨hq, hqe⟩
+--     · exact Or.inr (ih (Std.not_lt.1 hqe))
 
-theorem isChain_stupidSearch {ρ : Type} (pat : ρ) [ForwardPattern pat] [LawfulForwardPattern pat]
-    {s : Slice} (pos : s.Pos) : List.IsChain (fun p q => p.endPos = q.startPos) (stupidSearch pat pos) := by
-  fun_induction stupidSearch with
-  | case1 => simpa using List.IsChain.nil
-  | case2 p h endPos hend hlt ih =>
-    apply ih.cons_of_head? (fun st h => ?_)
-    simpa using (head?_stupidSearch _ _ _ h).symm
-  | case3 p h hend ih =>
-    apply ih.cons_of_head? (fun st h => ?_)
-    simpa using (head?_stupidSearch _ _ _ h).symm
+-- theorem lt_of_stupidSearch {ρ : Type} (pat : ρ) [ForwardPattern pat] [LawfulForwardPattern pat]
+--     {s : Slice} (pos : s.Pos) : ∀ st ∈ stupidSearch pat pos, st.startPos < st.endPos := by
+--   fun_induction stupidSearch with
+--   | case1 => simp
+--   | case2 p hp endPos hend hlt ih => simpa using ⟨hlt, ih⟩
+--   | case3 p hp hend ih => simpa
 
-theorem isMatchList_stupidSearch {ρ : Type} (pat : ρ) [ForwardPattern pat] [LawfulForwardPattern pat]
-    (s : Slice) : IsMatchList s (stupidSearch pat s.startPos) where
-  exists_le_and_lt p hp := exists_le_and_lt_stupidSearch _ _ _ (by simp) hp
-  lt := lt_of_stupidSearch _ _
-  isChain := isChain_stupidSearch _ _
+-- theorem isChain_stupidSearch {ρ : Type} (pat : ρ) [ForwardPattern pat] [LawfulForwardPattern pat]
+--     {s : Slice} (pos : s.Pos) : List.IsChain (fun p q => p.endPos = q.startPos) (stupidSearch pat pos) := by
+--   fun_induction stupidSearch with
+--   | case1 => simpa using List.IsChain.nil
+--   | case2 p h endPos hend hlt ih =>
+--     apply ih.cons_of_head? (fun st h => ?_)
+--     simpa using (head?_stupidSearch _ _ _ h).symm
+--   | case3 p h hend ih =>
+--     apply ih.cons_of_head? (fun st h => ?_)
+--     simpa using (head?_stupidSearch _ _ _ h).symm
+
+-- theorem isMatchList_stupidSearch {ρ : Type} (pat : ρ) [ForwardPattern pat] [LawfulForwardPattern pat]
+--     (s : Slice) : IsMatchList s (stupidSearch pat s.startPos) where
+--   exists_le_and_lt p hp := exists_le_and_lt_stupidSearch _ _ _ (by simp) hp
+--   lt := lt_of_stupidSearch _ _
+--   isChain := isChain_stupidSearch _ _
 
 theorem ForwardCharPredSearcher.step_eq_if
     {i : Std.Iter (α := ForwardCharPredSearcher p s) (SearchStep s)} :
@@ -434,32 +444,30 @@ theorem ForwardCharPredSearcher.rejected_mem_toList {p : Char → Bool} {s : Sli
   simp [toList_positions, mem_positionsFrom]
   grind
 
-theorem startsWith_charPred
+-- instance {p : Char → Bool} : LawfulToForwardSearcherForwardPattern p where
+--   reject_valid {s} l r := by
+--     simp
+--   match_valid {s} p := sorry
 
-instance {p : Char → Bool} : LawfulToForwardSearcherForwardPattern p where
-  reject_valid {s} l r := by
-    simp
-  match_valid {s} p := sorry
+-- instance {p : Char → Bool} : LawfulToForwardSearcher p where
+--   isMatchList s := by
+--     rw [ForwardCharPredSearcher.toList_toSearcher]
+--     simp [toList_positions]
+--     refine ⟨?_, fun st => ?_, ?_⟩
+--     · intro q hq
+--       simp only [List.mem_map, Subtype.exists, mem_positionsFrom, Pos.startPos_le, true_and]
+--       refine ⟨if p (q.get hq) then SearchStep.matched q (q.next hq)
+--         else SearchStep.rejected q (q.next hq), ⟨q, hq, by simp⟩, ?_⟩
+--       split <;> simp
+--     · simp [mem_positionsFrom]
+--       intro p hp
+--       split <;> rintro rfl <;> simp
+--     · apply List.isChain_map_of_isChain _ _ isChain_positionsFrom
+--       rintro ⟨a, ha⟩ ⟨b, hb⟩ rfl
+--       simp only
+--       split <;> split <;> simp
 
-instance {p : Char → Bool} : LawfulToForwardSearcher p where
-  isMatchList s := by
-    rw [ForwardCharPredSearcher.toList_toSearcher]
-    simp [toList_positions]
-    refine ⟨?_, fun st => ?_, ?_⟩
-    · intro q hq
-      simp only [List.mem_map, Subtype.exists, mem_positionsFrom, Pos.startPos_le, true_and]
-      refine ⟨if p (q.get hq) then SearchStep.matched q (q.next hq)
-        else SearchStep.rejected q (q.next hq), ⟨q, hq, by simp⟩, ?_⟩
-      split <;> simp
-    · simp [mem_positionsFrom]
-      intro p hp
-      split <;> rintro rfl <;> simp
-    · apply List.isChain_map_of_isChain _ _ isChain_positionsFrom
-      rintro ⟨a, ha⟩ ⟨b, hb⟩ rfl
-      simp only
-      split <;> split <;> simp
-
-instance {pat : Char → Bool} : LawfulForwardPattern pat := .defaultImplementation
+-- instance {pat : Char → Bool} : LawfulForwardPattern pat := .defaultImplementation
 
 end Pattern
 
